path_wp: add pure version, prove more powerful lemmas

theories/Dot/lr/path_wp.v
@@ -1,18 +1,78 @@
 From iris.proofmode Require Import tactics.
 From D Require Import iris_prelude.
-From D.Dot Require Import dlang_inst.
+From D.Dot Require Import dlang_inst rules.
 
 Implicit Types
          (L T U: ty) (v: vl) (e: tm) (d: dm) (ds: dms) (p : path)
-         (Γ : ctx) (ρ : vls).
+         (Γ : ctx) (ρ : env) (Pv : vl → Prop).
 
+(* Auxiliary. *)
 Lemma plength_subst_inv p s :
   plength p.|[s] = plength p.
 Proof. by elim: p => [v| p /= ->]. Qed.
 
+Lemma path2tm_subst p ρ: (path2tm p).|[ρ] = path2tm p.|[ρ].
+Proof. by elim: p => /= [//|p -> l]. Qed.
+
+(** * Pure path weakest precondition. *)
+Fixpoint path_wp_pure p Pv : Prop :=
+  match p with
+  | pself p l => path_wp_pure p (λ v, ∃ w, v @ l ↘ dvl w ∧ Pv w)
+  | pv vp => Pv vp
+  end.
+
+Global Instance Proper_pwp_pure: Proper ((=) ==> pointwise_relation _ iff ==> iff) path_wp_pure.
+Proof.
+  (* The induction works best in this shape, but this instance is best kept local. *)
+  have Proper_pwp_2: ∀ p, Proper (pointwise_relation _ iff ==> iff) (path_wp_pure p).
+  elim; solve_proper.
+  solve_proper.
+Qed.
+
+Lemma path_wp_pure_wand {Pv1 Pv2 p}:
+  path_wp_pure p Pv1 →
+  (∀ v, Pv1 v → Pv2 v) →
+  path_wp_pure p Pv2.
+Proof.
+  elim: p Pv1 Pv2 => /= [v|p IHp l] Pv1 Pv2 Hp Hwand;
+    first by apply Hwand.
+  apply: (IHp _ _ Hp) => {IHp Hp} v [vq [??]].
+  eauto.
+Qed.
+
+Lemma path_wp_pure_eq p Pv :
+  path_wp_pure p Pv ↔ ∃ v, path_wp_pure p (λ w, w = v) ∧ Pv v.
+Proof.
+  elim: p Pv => [ v | p IHp l ] Pv /=; split.
+  - eauto.
+  - by destruct 1 as (w & <- & ?).
+  - rewrite IHp; intros (v & Hp & w & ?&?).
+    eexists w; split; last by [].
+    apply (path_wp_pure_wand Hp).
+    intros v' ->; exists w; eauto.
+  - setoid_rewrite IHp; intros; ev; subst; eauto.
+Qed.
+
+Lemma path_wp_pure_det {p v1 v2}:
+  path_wp_pure p (λ w, w = v1) →
+  path_wp_pure p (λ w, w = v2) →
+  v1 = v2.
+Proof.
+  elim: p v1 v2 => [v /=| p /= IHp l //] v1 v2; first by intros <- <-.
+  rewrite !path_wp_pure_eq; intros (w1 & Hp1 & ?) (w2 & Hp2 & ?);
+    move: (IHp _ _ Hp1 Hp2) => ?; ev; simplify_eq.
+  by objLookupDet.
+Qed.
+
+Lemma path_wp_pure_swap p u :
+  path_wp_pure p (λ w, u = w) ↔
+  path_wp_pure p (λ w, w = u).
+Proof. split => Hp; exact: path_wp_pure_wand. Qed.
+
 Section path_wp.
   Context `{HdlangG: dlangG Σ}.
   Implicit Types (φ : vl -d> iPropO Σ).
+  Notation path_wp_purel p Pv := (⌜path_wp_pure p Pv⌝%I : iProp Σ).
 
   (** A simplified variant of weakest preconditions for path evaluation.
       The difference is that path evaluation is completely pure, and
@@ -39,7 +99,39 @@ Section path_wp.
     (∀ v, Persistent (φ v)) → Persistent (path_wp p φ).
   Proof. elim: p φ => *; apply _. Qed.
 
-  Lemma strong_path_wp_wand φ1 φ2 p:
+  Global Instance Proper_pwp: Proper ((=) ==> pointwise_relation _ (≡) ==> (≡)) path_wp.
+  Proof.
+    (* The induction works best in this shape, but this instance is best kept local. *)
+    have Proper_pwp_2: ∀ p, Proper (pointwise_relation _ (≡) ==> (≡)) (path_wp p).
+    elim; solve_proper.
+    solve_proper.
+  Qed.
+
+  Lemma path_wp_pureable p Pv:
+    path_wp p (λ v, ⌜Pv v⌝) ⊣⊢ path_wp_purel p Pv.
+  Proof.
+    elim: p Pv => /= [//|p IHp l] Pv.
+    by rewrite -{}IHp; f_equiv => v; iIntros "!% /=".
+  Qed.
+
+  Global Instance path_wp_pureableI p Pv :
+    IntoPure (path_wp p (λ v, ⌜Pv v⌝))%I (path_wp_pure p Pv).
+  Proof. by rewrite /IntoPure path_wp_pureable. Qed.
+  Global Instance path_wp_pureableF p Pv :
+    FromPure false (path_wp p (λ v, ⌜Pv v⌝))%I (path_wp_pure p Pv).
+  Proof. by rewrite /FromPure/= path_wp_pureable. Qed.
+
+  Lemma path_wp_det p v1 v2:
+    path_wp p (λ w, ⌜ w = v1 ⌝) -∗
+    path_wp p (λ w, ⌜ w = v2 ⌝) -∗
+    ⌜ v1 = v2 ⌝: iProp Σ.
+  Proof. iIntros "!%". exact: path_wp_pure_det. Qed.
+
+  Lemma path_wp_swap p u :
+    path_wp p (λ w, ⌜u = w⌝) ⊣⊢ path_wp p (λ w, ⌜w = u⌝).
+  Proof. iIntros "!%". by rewrite /= path_wp_pure_swap. Qed.
+
+  Lemma path_wp_wand φ1 φ2 p:
     path_wp p φ1 -∗
     (∀ v, φ1 v -∗ φ2 v) -∗
     path_wp p φ2.
@@ -47,17 +139,8 @@ Section path_wp.
     elim: p φ1 φ2 => /= [v|p IHp l] ??; iIntros "H1 Hwand";
       first by iApply "Hwand".
     iApply (IHp with "H1").
-    iIntros (v) "H"; iDestruct "H" as (vq Hl) "?".
+    iIntros (v); iDestruct 1 as (vq Hl) "?".
     iExists vq; iFrame (Hl). by iApply "Hwand".
-  Qed.
-
-  Lemma path_wp_wand φ1 φ2 p:
-    path_wp p φ1 -∗
-    (∀ v, φ1 v -∗ φ2 v) -∗
-    path_wp p φ2.
-  Proof.
-    iIntros "Hp1 Hwand".
-    by iApply (strong_path_wp_wand with "Hp1").
   Qed.
 
   Lemma path_wp_eq p φ :
@@ -76,27 +159,7 @@ Section path_wp.
       iDestruct "H" as (w) "[Hp Hw]".
       iDestruct "Hp" as (v) "[Hp Hl]".
       iExists v; iSplit; first done.
-      iDestruct "Hl" as (w') "[Hl Heqw]".
-      iExists w'; iSplit; first done.
-      by iDestruct "Heqw" as %->.
-  Qed.
-
-  Lemma path_wp_det p v1 v2:
-    path_wp p (λ w, ⌜ w = v1 ⌝) -∗
-    path_wp p (λ w, ⌜ w = v2 ⌝) -∗
-    ⌜ v1 = v2 ⌝: iProp Σ.
-  Proof.
-    elim: p v1 v2 => [v /=| p /= IHp l //] v1 v2;
-      first by iIntros (<- <-).
-    rewrite !path_wp_eq.
-    iIntros "H1 H2".
-    iDestruct "H1" as (w1) "[H1 Hl1]".
-    iDestruct "H2" as (w2) "[H2 Hl2]".
-    iDestruct (IHp with "H1 H2") as "Heq".
-    iDestruct "Heq" as %<-.
-    iDestruct "Hl1" as (vq1 Hl1) "Heq1".
-    iDestruct "Hl2" as (vq2 Hl2) "Heq2".
-    objLookupDet. iDestruct "Heq1" as %->. by [].
+      iDestruct "Hl" as %(w' & Hl & ->). auto.
   Qed.
 
   Lemma path_wp_later_swap p φ:
@@ -117,4 +180,33 @@ Section path_wp.
     elim: i => [// | i /= <-].
     rewrite path_wp_later_swap. by [].
   Qed.
+
+  Global Instance Plain_path_wp p φ (H : (∀ v, Plain (φ v))) :
+    Plain (path_wp p φ).
+  Proof.
+    elim: p φ H => /= [//|p IHp l] φ H; rewrite path_wp_eq /Plain.
+    iDestruct 1 as (v) "#[Heq H]"; iDestruct "H" as (w Hl) "#H".
+    iModIntro. repeat (iExists _; iSplit => //).
+  Qed.
+
+  Lemma path_wp_exec_pure p v :
+    path_wp_pure p (λ v0 : vl, v0 = v)
+    → PureExec True (plength p) (path2tm p) (tv v).
+  Proof.
+    elim: p v => [w|p IHp l] v; rewrite /PureExec/=.
+    by intros -> _; constructor.
+    rewrite path_wp_pure_eq; intros (vp & Hp & vq & Hlook & ->) _.
+    move: (IHp _ Hp) => Hpure.
+    eapply nsteps_r.
+    - by apply (pure_step_nsteps_ctx (fill_item (ProjCtx l))), Hpure.
+    - apply nsteps_once_inv, pure_tproj, Hlook.
+  Qed.
+
+  Lemma path_wp_exec p v :
+    path_wp p (λ w, ⌜ w = v ⌝) ⊢@{iPropI Σ}
+    ⌜ PureExec True (plength p) (path2tm p) (tv v) ⌝.
+  Proof. iIntros "!%". apply path_wp_exec_pure. Qed.
+
+  Global Instance path_wp_timeless p Pv: Timeless (path_wp p (λ v, ⌜Pv v⌝))%I.
+  Proof. rewrite path_wp_pureable. apply _. Qed.
 End path_wp.
